compiler/backend/proofs/data_to_wordProofScript.sml
@@ -5930,6 +5930,14 @@ val word_cmp_Less_word_cmp_res = prove(
   \\ fs [word_cmp_res_def,asmSemTheory.word_cmp_def]
   \\ rw [] \\ fs [WORD_LT] \\ fs [word_msb_def,word_index,dimword_def]);
 
+val word_cmp_NotLess_word_cmp_res = prove(
+  ``!i i'. good_dimindex (:'a) ==>
+           (word_cmp NotLess (1w:'a word) (word_cmp_res i i') <=> (i <= i'))``,
+  rw [] \\ fs [labPropsTheory.good_dimindex_def]
+  \\ fs [word_cmp_res_def,asmSemTheory.word_cmp_def]
+  \\ rw [] \\ fs [WORD_LT] \\ fs [word_msb_def,word_index,dimword_def]
+  \\ intLib.COOPER_TAC);
+
 val IMP_spt_eq = store_thm("IMP_spt_eq",
   ``wf t1 /\ wf t2 /\ (∀n. lookup n t1 = lookup n t2) ==> (t1 = t2)``,
   metis_tac [spt_eq_thm]);
@@ -6083,97 +6091,143 @@ val th = Q.store_thm("assign_Less",
   \\ fs [lookup_inter_alt,SUBSET_DEF]
   \\ rw [] \\ fs [domain_inter] \\ res_tac);
 
-val th = Q.store_thm("assign_GreaterEq",
-  `op = GreaterEq ==> ^assign_thm_goal`,
-  rpt strip_tac \\ drule (evaluate_GiveUp |> GEN_ALL) \\ rw [] \\ fs []
-  \\ `t.termdep <> 0` by fs[]
-  \\ imp_res_tac state_rel_cut_IMP \\ pop_assum mp_tac
-  \\ qpat_x_assum `state_rel c l1 l2 s t [] locs` kall_tac \\ strip_tac
-  \\ cheat (* update for bignums *) (*
-   (imp_res_tac get_vars_IMP_LENGTH \\ fs [] \\ rw []
-    \\ fs [do_app] \\ rfs [] \\ every_case_tac \\ fs []
-    \\ clean_tac \\ fs []
-    \\ imp_res_tac state_rel_get_vars_IMP
-    \\ fs [LENGTH_EQ_2] \\ clean_tac
-    \\ fs [get_var_def]
-    \\ fs [state_rel_thm] \\ eval_tac
-    \\ full_simp_tac std_ss [GSYM APPEND_ASSOC]
-    \\ rpt_drule (memory_rel_get_vars_IMP |> GEN_ALL)
-    \\ strip_tac
-    \\ rpt_drule memory_rel_Number_LESS \\ rw [] \\ fs []
-    \\ fs [wordSemTheory.get_vars_def] \\ every_case_tac
-    \\ fs [wordSemTheory.get_var_imm_def] \\ clean_tac
-    \\ fs [assign_def] \\ eval_tac
-    \\ fs [wordSemTheory.get_var_imm_def,asmSemTheory.word_cmp_def]
-    \\ fs [intLib.COOPER_PROVE `` i >= j:int <=> ~(i < j)``]
-    \\ IF_CASES_TAC \\ fs []
-    \\ fs [lookup_insert,adjust_var_11] \\ rw [] \\ fs []
-    \\ full_simp_tac std_ss [GSYM APPEND_ASSOC]
-    \\ match_mp_tac memory_rel_insert \\ fs []
-    \\ TRY (match_mp_tac memory_rel_Boolv_T \\ fs [] \\ NO_TAC)
-    \\ TRY (match_mp_tac memory_rel_Boolv_F \\ fs [] \\ NO_TAC)) *));
-
-val th = Q.store_thm("assign_Greater",
-  `op = Greater ==> ^assign_thm_goal`,
-  rpt strip_tac \\ drule (evaluate_GiveUp |> GEN_ALL) \\ rw [] \\ fs []
-  \\ `t.termdep <> 0` by fs[]
-  \\ imp_res_tac state_rel_cut_IMP \\ pop_assum mp_tac
-  \\ qpat_x_assum `state_rel c l1 l2 s t [] locs` kall_tac \\ strip_tac
-  \\ cheat (* update for bignums *) (*
-   (imp_res_tac get_vars_IMP_LENGTH \\ fs [] \\ rw []
-    \\ fs [do_app] \\ rfs [] \\ every_case_tac \\ fs []
-    \\ clean_tac \\ fs []
-    \\ imp_res_tac state_rel_get_vars_IMP
-    \\ fs [LENGTH_EQ_2] \\ clean_tac
-    \\ fs [get_var_def]
-    \\ fs [state_rel_thm] \\ eval_tac
-    \\ full_simp_tac std_ss [GSYM APPEND_ASSOC]
-    \\ rpt_drule (memory_rel_get_vars_IMP |> GEN_ALL)
-    \\ strip_tac
-    \\ rpt_drule memory_rel_Number_LESS_EQ \\ rw [] \\ fs []
-    \\ fs [wordSemTheory.get_vars_def] \\ every_case_tac
-    \\ fs [wordSemTheory.get_var_imm_def] \\ clean_tac
-    \\ fs [assign_def] \\ eval_tac
-    \\ fs [wordSemTheory.get_var_imm_def,asmSemTheory.word_cmp_def]
-    \\ simp [word_less_lemma1]
-    \\ fs [intLib.COOPER_PROVE `` i > j:int <=> ~(i <= j)``]
-    \\ IF_CASES_TAC \\ fs []
-    \\ fs [lookup_insert,adjust_var_11] \\ rw [] \\ fs []
-    \\ full_simp_tac std_ss [GSYM APPEND_ASSOC]
-    \\ match_mp_tac memory_rel_insert \\ fs []
-    \\ TRY (match_mp_tac memory_rel_Boolv_T \\ fs [] \\ NO_TAC)
-    \\ TRY (match_mp_tac memory_rel_Boolv_F \\ fs [] \\ NO_TAC)) *));
-
 val th = Q.store_thm("assign_LessEq",
   `op = LessEq ==> ^assign_thm_goal`,
   rpt strip_tac \\ drule (evaluate_GiveUp |> GEN_ALL) \\ rw [] \\ fs []
   \\ `t.termdep <> 0` by fs[]
-  \\ imp_res_tac state_rel_cut_IMP \\ pop_assum mp_tac
-  \\ qpat_x_assum `state_rel c l1 l2 s t [] locs` kall_tac \\ strip_tac
-  \\ cheat (* update for bignums *) (*
-   (imp_res_tac get_vars_IMP_LENGTH \\ fs [] \\ rw []
-    \\ fs [do_app] \\ rfs [] \\ every_case_tac \\ fs []
-    \\ clean_tac \\ fs []
-    \\ imp_res_tac state_rel_get_vars_IMP
-    \\ fs [LENGTH_EQ_2] \\ clean_tac
-    \\ fs [get_var_def]
-    \\ fs [state_rel_thm] \\ eval_tac
-    \\ full_simp_tac std_ss [GSYM APPEND_ASSOC]
-    \\ rpt_drule (memory_rel_get_vars_IMP |> GEN_ALL)
-    \\ strip_tac
-    \\ rpt_drule memory_rel_Number_LESS_EQ \\ rw [] \\ fs []
-    \\ fs [wordSemTheory.get_vars_def] \\ every_case_tac
-    \\ fs [wordSemTheory.get_var_imm_def] \\ clean_tac
-    \\ fs [assign_def] \\ eval_tac
+  \\ imp_res_tac state_rel_cut_IMP \\ pop_assum mp_tac \\ strip_tac
+  \\ imp_res_tac get_vars_IMP_LENGTH \\ fs [] \\ rw []
+  \\ fs [do_app] \\ rfs [] \\ every_case_tac \\ fs []
+  \\ clean_tac \\ fs []
+  \\ imp_res_tac state_rel_get_vars_IMP
+  \\ fs [LENGTH_EQ_2] \\ clean_tac
+  \\ fs [get_var_def]
+  \\ fs [Boolv_def] \\ rveq \\ fs [GSYM Boolv_def]
+  \\ qpat_assum `state_rel c l1 l2 x t [] locs`
+           (assume_tac o REWRITE_RULE [state_rel_thm])
+  \\ eval_tac
+  \\ full_simp_tac std_ss [GSYM APPEND_ASSOC]
+  \\ rpt_drule (memory_rel_get_vars_IMP |> GEN_ALL)
+  \\ strip_tac
+  \\ rpt_drule memory_rel_Number_cmp
+  \\ strip_tac \\ fs [] \\ rveq
+  \\ fs [get_vars_SOME_IFF_data,get_vars_SOME_IFF]
+  \\ fs [wordSemTheory.get_var_def]
+  \\ fs [assign_def,list_Seq_def] \\ eval_tac
+  \\ fs [lookup_insert,wordSemTheory.get_var_def,wordSemTheory.get_var_imm_def,
+         word_cmp_Test_1,word_bit_or]
+  \\ IF_CASES_TAC THEN1
+   (fs [lookup_insert,state_rel_thm]
     \\ fs [wordSemTheory.get_var_imm_def,asmSemTheory.word_cmp_def]
+    \\ `i <= i' <=> w1 <= w2` by
+          (fs [integerTheory.INT_LE_LT,WORD_LESS_OR_EQ] \\ NO_TAC)
     \\ fs [WORD_NOT_LESS,intLib.COOPER_PROVE ``~(i < j) <=> j <= i:int``]
     \\ simp [word_less_lemma1]
     \\ IF_CASES_TAC \\ fs []
     \\ fs [lookup_insert,adjust_var_11] \\ rw [] \\ fs []
+    \\ simp[inter_insert_ODD_adjust_set,GSYM Boolv_def]
     \\ full_simp_tac std_ss [GSYM APPEND_ASSOC]
     \\ match_mp_tac memory_rel_insert \\ fs []
-    \\ TRY (match_mp_tac memory_rel_Boolv_T \\ fs [] \\ NO_TAC)
-    \\ TRY (match_mp_tac memory_rel_Boolv_F \\ fs [] \\ NO_TAC)) *));
+    \\ TRY (match_mp_tac memory_rel_Boolv_T \\ fs [])
+    \\ TRY (match_mp_tac memory_rel_Boolv_F \\ fs [])
+    \\ match_mp_tac (GEN_ALL memory_rel_zero_space)
+    \\ metis_tac [])
+  \\ pop_assum mp_tac
+  \\ rpt_drule (Compare_code_thm |> INST_TYPE [``:'b``|->``:'ffi``])
+  \\ ho_match_mp_tac (METIS_PROVE []
+         ``((!x1 x2 x3. (b2 ==> b0 x1 x2 x3) ==> b1 x1 x2 x3) ==> b3) ==>
+           ((!x1 x2 x3. b0 x1 x2 x3 ==> b1 x1 x2 x3) ==> b2 ==> b3)``)
+  \\ strip_tac
+  \\ fs [wordSemTheory.get_vars_def,wordSemTheory.get_var_def,lookup_insert,
+         wordSemTheory.bad_dest_args_def,wordSemTheory.find_code_def]
+  \\ `lookup Compare_location t.code = SOME (3,Compare_code c)` by
+       (fs [state_rel_def,code_rel_def,stubs_def] \\ NO_TAC)
+  \\ fs [wordSemTheory.add_ret_loc_def]
+  \\ fs [bvi_to_dataTheory.op_requires_names_def,
+         bvi_to_dataTheory.op_space_reset_def]
+  \\ TOP_CASE_TAC THEN1
+   (Cases_on `names_opt` \\ fs []
+    \\ fs [cut_state_opt_def,cut_state_def]
+    \\ Cases_on `dataSem$cut_env x' s.locals` \\ fs []
+    \\ qpat_x_assum `state_rel c l1 l2 s t [] locs` assume_tac
+    \\ rpt_drule cut_env_IMP_cut_env
+    \\ CCONTR_TAC \\ fs [get_names_def]
+    \\ fs [wordSemTheory.cut_env_def,SUBSET_DEF])
+  \\ fs []
+  \\ qpat_abbrev_tac `t1 = wordSem$call_env _ _`
+  \\ first_x_assum (qspecl_then [`t1`,`l`,`n`] mp_tac)
+  \\ impl_tac THEN1
+   (unabbrev_all_tac
+    \\ fs [wordSemTheory.call_env_def,wordSemTheory.push_env_def,
+           wordSemTheory.dec_clock_def]
+    \\ pairarg_tac \\ fs []
+    \\ fs [fromList2_def,lookup_insert]
+    \\ fs [state_rel_def,code_rel_def,stubs_def]
+    \\ fs [memory_rel_def,word_ml_inv_def,heap_in_memory_store_def]
+    \\ fs [dimword_LESS_MustTerminate_limit]
+    \\ rpt strip_tac \\ simp [] \\ NO_TAC)
+  \\ strip_tac \\ fs []
+  \\ `?t2. pop_env t1 = SOME t2 /\ domain t2.locals = domain x'` by
+   (unabbrev_all_tac
+    \\ fs [wordSemTheory.call_env_def,wordSemTheory.push_env_def,
+           wordSemTheory.pop_env_def] \\ pairarg_tac \\ fs []
+    \\ imp_res_tac env_to_list_lookup_equiv
+    \\ fs [domain_lookup,EXTENSION,lookup_fromAList] \\ NO_TAC)
+  \\ fs []
+  \\ fs [lookup_insert,word_cmp_NotLess_word_cmp_res]
+  \\ rw [] \\ fs []
+  \\ unabbrev_all_tac
+  \\ fs [wordSemTheory.pop_env_def,wordSemTheory.call_env_def,
+         wordSemTheory.push_env_def,wordSemTheory.dec_clock_def]
+  \\ pairarg_tac \\ fs [] \\ rveq \\ fs []
+  \\ simp [state_rel_thm]
+  \\ fs [lookup_insert]
+  \\ rpt_drule env_to_list_cut_env_IMP \\ fs []
+  \\ disch_then kall_tac
+  \\ fs [lookup_insert,FAPPLY_FUPDATE_THM,adjust_var_11,FLOOKUP_UPDATE]
+  \\ fs [inter_insert_ODD_adjust_set]
+  \\ fs [wordSemTheory.cut_env_def] \\ rveq
+  \\ conj_tac
+  \\ TRY (fs [lookup_inter,lookup_insert,adjust_set_def,fromAList_def] \\ NO_TAC)
+  \\ `domain (adjust_set (get_names names_opt)) SUBSET domain t.locals` by
+   (Cases_on `names_opt` \\ fs [get_names_def]
+    \\ fs [SUBSET_DEF,domain_lookup]
+    \\ rw [] \\ res_tac \\ fs []
+    \\ rveq \\ fs [lookup_ODD_adjust_set] \\ NO_TAC)
+  \\ `domain (adjust_set x.locals) SUBSET
+      domain (inter t.locals (adjust_set (get_names names_opt)))` by
+   (fs [SUBSET_DEF,domain_lookup,lookup_inter_alt] \\ rw []
+    \\ Cases_on `names_opt` \\ fs [get_names_def]
+    \\ fs [SUBSET_DEF,domain_lookup]
+    \\ fs [cut_state_opt_def,cut_state_def,cut_env_def]
+    \\ qpat_x_assum `_ = SOME x` mp_tac
+    \\ IF_CASES_TAC \\ fs [] \\ rw [] \\ fs [adjust_set_inter]
+    \\ fs [lookup_inter_alt,domain_lookup] \\ NO_TAC)
+  \\ `!n. IS_SOME (lookup n x.locals) ==>
+          n ∈ domain (get_names names_opt) /\
+          IS_SOME (lookup (adjust_var n) t.locals)` by
+   (qx_gen_tac `k` \\ disch_then assume_tac
+    \\ Cases_on `lookup k x.locals` \\ fs []
+    \\ Cases_on `names_opt` \\ fs [get_names_def]
+    \\ fs [SUBSET_DEF,domain_lookup]
+    \\ fs [cut_state_opt_def,cut_state_def,cut_env_def]
+    \\ qpat_x_assum `_ = SOME x` mp_tac
+    \\ IF_CASES_TAC \\ fs [] \\ rw [] \\ fs [adjust_set_inter]
+    \\ fs [lookup_inter_alt,domain_lookup] \\ NO_TAC)
+  \\ conj_tac
+  \\ TRY (rw [] \\ once_rewrite_tac [lookup_inter_alt]
+          \\ fs [lookup_insert,adjust_var_IN_adjust_set] \\ NO_TAC)
+  \\ full_simp_tac std_ss [GSYM APPEND_ASSOC]
+  \\ match_mp_tac memory_rel_insert \\ fs [inter_insert_ODD_adjust_set_alt]
+  \\ match_mp_tac (GEN_ALL memory_rel_zero_space)
+  \\ qexists_tac `x.space`
+  \\ TRY (match_mp_tac memory_rel_Boolv_T)
+  \\ TRY (match_mp_tac memory_rel_Boolv_F) \\ fs []
+  \\ qsuff_tac `inter (inter t.locals (adjust_set (get_names names_opt)))
+                 (adjust_set x.locals) = inter t.locals (adjust_set x.locals)`
+  \\ asm_simp_tac std_ss [] \\ fs []
+  \\ fs [lookup_inter_alt,SUBSET_DEF]
+  \\ rw [] \\ fs [domain_inter] \\ res_tac);
 
 val th = Q.store_thm("assign_Equal",
   `op = Equal ==> ^assign_thm_goal`,
@@ -7813,6 +7867,10 @@ val assign_thm = Q.store_thm("assign_thm",
   \\ Cases_on `?i. op = Global i` \\ fs []
   THEN1 (fs [do_app] \\ every_case_tac \\ fs [])
   \\ Cases_on `?i. op = SetGlobal i` \\ fs []
+  THEN1 (fs [do_app] \\ every_case_tac \\ fs [])
+  \\ Cases_on `op = Greater` \\ fs []
+  THEN1 (fs [do_app] \\ every_case_tac \\ fs [])
+  \\ Cases_on `op = GreaterEq` \\ fs []
   THEN1 (fs [do_app] \\ every_case_tac \\ fs [])
   \\ map_every (fn th =>
          (Cases_on `^(th |> concl |> dest_imp |> #1)` THEN1 (fs []
